tests/binders.v
@@ -2,17 +2,18 @@ Require Import Mtac2.Datatypes Mtac2.Mtac2.
 
 Example nu_new_name_works : forall x:nat, 0 <= x.
 MProof.
-  M.nu "x" mNone (fun y=> M.abs_fun y (le_0_n y)).
+  M.nu (TheName "x") mNone (fun y=> M.abs_fun y (le_0_n y)).
 Qed.
 
 Example nu_existing_name_fails (x: nat) : forall y:nat, 0 <= y.
 MProof.
-  (mtry M.nu "x" mNone (fun y=>M.abs_fun y (le_0_n y)) with NameExistsInContext "x"=>M.ret _ end)%MC.
+Mtac Do Set_Debug_Exceptions.
+  (mtry M.nu (TheName "x") mNone (fun y=>M.abs_fun y (le_0_n y)) with NameExistsInContext (TheName "x")=>M.ret _ end)%MC.
 Abort.
 
 Example nu_returning_x_fails (x: nat) : forall y:nat, 0 <= y.
 MProof.
-  (mtry M.nu "z" mNone (fun y=>M.ret y) with VarAppearsInValue => M.ret _ end)%MC.
+  (mtry M.nu (TheName "z") mNone (fun y=>M.ret y) with VarAppearsInValue => M.ret _ end)%MC.
 Abort.
 
 Example fresh_nu : True.
